<?xml version="1.0"?>
<rdf:RDF xmlns="http://w3id.org/claimont#"
     xml:base="http://w3id.org/claimont"
     xmlns:owl="http://www.w3.org/2002/07/owl#"
     xmlns:rdf="http://www.w3.org/1999/02/22-rdf-syntax-ns#"
     xmlns:rdfs="http://www.w3.org/2000/01/rdf-schema#"
	 xmlns:skos="http://www.w3.org/2004/02/skos/core#"
	 xmlns:schema="http://schema.org/"
	 xmlns:dcterms="http://purl.org/dc/terms/"
	 xmlns:lrml="http://docs.oasis-open.org/legalruleml/ns/v1.0/">

	<owl:Ontology rdf:about="http://w3id.org/claimont">
		<dcterms:title xml:lang="en">Claim Ontology</dcterms:title>
		<dcterms:description xml:lang="en">An ontology for describing claims and their substantiation.</dcterms:description>
	</owl:Ontology>

	<!-- Classes with Definitions -->
	<owl:Class rdf:about="http://w3id.org/claimont#Claim">
		<rdfs:label>Claim</rdfs:label>
		<skos:definition>A defeasible statement about a thing.</skos:definition>
		<rdfs:comment>A Claim may comprise other Claims.</rdfs:comment>	
		<rdfs:subClassOf rdf:resource="http://docs.oasis-open.org/legalruleml/ns/v1.0/Statement"/>
		<rdfs:subClassOf>
			<owl:Restriction>
				<owl:onProperty rdf:resource="http://w3id.org/claimont#hasSubject"/>
				<owl:allValuesFrom rdf:resource="http://w3id.org/claimont#Subject"/>
			</owl:Restriction>
		</rdfs:subClassOf>
		<rdfs:subClassOf>
			<owl:Restriction>
				<owl:onProperty rdf:resource="http://w3id.org/claimont#isMadeBy"/>
				<owl:allValuesFrom rdf:resource="http://w3id.org/claimont#Claimant"/>
			</owl:Restriction>
		</rdfs:subClassOf>			
	</owl:Class>	
	
	<owl:Class rdf:about="http://w3id.org/claimont#Claimant">
		<rdfs:label>Claimant</rdfs:label>
		<skos:definition>An entity (e.g., a person, an organisation or a system) that makes a claim.</skos:definition>
	</owl:Class>
	
	<owl:Class rdf:about="http://w3id.org/claimont#Subject">
		<rdfs:label>Subject</rdfs:label>
		<skos:definition>The thing about which a statement (i.e., a claim or an attestation) is made.</skos:definition>
		<owl:equivalentClass rdf:resource="http://www.w3.org/2002/07/owl#Thing"/>
	</owl:Class>
	
	<owl:Class rdf:about="http://w3id.org/claimont#Predicate">
		<rdfs:label>Predicate</rdfs:label>
		<skos:definition>The characteristic, attribute, or relationship asserted about the subject of a claim or an attestation.</skos:definition>
	</owl:Class>
	
	<owl:Class rdf:about="http://w3id.org/claimont#Object">
		<rdfs:label>Object</rdfs:label>
		<skos:definition>The target or value associated with the predicate of a claim or an attestation.</skos:definition>
	</owl:Class>
	
	<owl:Class rdf:about="http://w3id.org/claimont#Substantiation">
		<rdfs:label>Substantiation</rdfs:label>
		<skos:definition>A thing presented in support of the truthfulness of a claim.</skos:definition>
	</owl:Class>

	<owl:Class rdf:about="http://w3id.org/claimont#IdentityClaim">
		<rdfs:subClassOf rdf:resource="#Claim"/>
		<rdfs:label>Identity Claim</rdfs:label>
		<skos:definition>A statement made by a claimant about their identity, usually with reference to some identification system.</skos:definition>
	</owl:Class>

	<owl:Class rdf:about="http://w3id.org/claimont#Attestation">
		<rdfs:subClassOf rdf:resource="#Substantiation"/>
		<rdfs:subClassOf rdf:resource="http://docs.oasis-open.org/legalruleml/ns/v1.0/Statement"/>
		<rdfs:subClassOf>
			<owl:Restriction>
				<owl:onProperty rdf:resource="http://w3id.org/claimont#hasSubject"/>
				<owl:allValuesFrom rdf:resource="http://w3id.org/claimont#Claim"/>
			</owl:Restriction>
		</rdfs:subClassOf>		
		<rdfs:subClassOf>
			<owl:Restriction>
				<owl:onProperty rdf:resource="http://w3id.org/claimont#isMadeBy"/>
				<owl:allValuesFrom rdf:resource="http://w3id.org/claimont#Attester"/>
			</owl:Restriction>
		</rdfs:subClassOf>		
		<rdfs:label>Attestation</rdfs:label>
		<skos:definition>An indefeasible statement, usually formal, made by an entity according to which they have witnessed or been presented with sufficient evidence to consider a specific claim made by another entity as truthful or accurate.</skos:definition>
		<rdfs:comment>A verifier's statement is an example of an attestation.</rdfs:comment>
	</owl:Class>
	
	<owl:Class rdf:about="http://w3id.org/claimont#Attester">
		<rdfs:label>Attester</rdfs:label>
		<skos:definition>An entity (e.g., a person, an organisation or a system) that makes an attestation.</skos:definition>
	</owl:Class>
	
	<owl:Class rdf:about="http://w3id.org/claimont#Report">
		<rdfs:subClassOf rdf:resource="#Claim"/>
		<rdfs:label>Report</rdfs:label>
		<skos:definition>A claim made according to some specification.</skos:definition>
	</owl:Class>

	<!-- Disjoint Classes -->
	<owl:AllDisjointClasses>
		<owl:members rdf:parseType="Collection">
			<owl:Class rdf:about="#Claim"/>
			<owl:Class rdf:about="#Substantiation"/>
		</owl:members>
	</owl:AllDisjointClasses>	

	<!-- Properties -->

	<owl:ObjectProperty rdf:about="http://w3id.org/claimont#isMadeBy">
		<rdfs:label>isMadeBy</rdfs:label>
		<rdfs:comment>This property is used on the Claim and Attestation classes. For a Claim the value assigned to this property must be a Claimant; for an Attestation the value must be an Attester. This is enforced by owl:Restriction (see the definitions of the Claim and Attestation classes.)</rdfs:comment>
	</owl:ObjectProperty>
	
	<owl:ObjectProperty rdf:about="http://w3id.org/claimont#hasSubject">
		<rdfs:label>hasSubject</rdfs:label>
		<rdfs:comment>This property is used on the Claim and Attestation classes. For a Claim the value assigned to this property must be a Subject; for an Attestation the value must be a Claim. This is enforced by owl:Restriction (see the definitions of the Claim and Attestation classes.)</rdfs:comment>
	</owl:ObjectProperty>	

	<owl:ObjectProperty rdf:about="http://w3id.org/claimont#hasPredicate">
		<rdfs:label>hasPredicate</rdfs:label>
		<rdfs:domain rdf:resource="#Claim"/>
		<rdfs:range rdf:resource="#Predicate"/>
	</owl:ObjectProperty>
	
	<owl:ObjectProperty rdf:about="http://w3id.org/claimont#hasObject">
		<rdfs:label>hasObject</rdfs:label>
		<rdfs:domain rdf:resource="#Claim"/>
		<rdfs:range rdf:resource="#Object"/>
	</owl:ObjectProperty>
	
	<owl:ObjectProperty rdf:about="http://w3id.org/claimont#comprisesClaims">
		<rdfs:label>comprisesClaims</rdfs:label>
		<rdfs:domain rdf:resource="#Claim"/>
		<rdfs:range rdf:resource="#Claim"/>
	</owl:ObjectProperty>	
	
	<owl:ObjectProperty rdf:about="http://w3id.org/claimont#isSupportedBy">
		<rdfs:domain rdf:resource="#Claim"/>
		<rdfs:range rdf:resource="#Substantiation"/>
		 <rdfs:label>isSupportedBy</rdfs:label>
		<skos:definition>Indicates that a claim is backed or reinforced by some form of substantiation or evidence.</skos:definition>
		<owl:inverseOf rdf:resource="#supports"/>		
	</owl:ObjectProperty>

	<owl:ObjectProperty rdf:about="http://w3id.org/claimont#supports">
		<rdfs:domain rdf:resource="#Substantiation"/>
		<rdfs:range rdf:resource="#Claim"/>
		<rdfs:label>supports</rdfs:label>
		<skos:definition>Indicates that a substantiation provides evidence or backing for a particular claim.</skos:definition> 
		<owl:inverseOf rdf:resource="#isSupportedBy"/>
	</owl:ObjectProperty>	

</rdf:RDF>

