@prefix : <http://w3id.org/claimont#> .
@prefix dcterms: <http://purl.org/dc/terms/> .
@prefix lrml: <http://docs.oasis-open.org/legalruleml/ns/v1.0/> .
@prefix owl: <http://www.w3.org/2002/07/owl#> .
@prefix rdf: <http://www.w3.org/1999/02/22-rdf-syntax-ns#> .
@prefix rdfs: <http://www.w3.org/2000/01/rdf-schema#> .
@prefix skos: <http://www.w3.org/2004/02/skos/core#> .

<http://w3id.org/claimont> a owl:Ontology ;
    dcterms:description "An ontology for describing claims and their substantiation."@en ;
    dcterms:title "Claim Ontology"@en .

:Attestation a owl:Class ;
    rdfs:label "Attestation" ;
    rdfs:comment "A verifier's statement is an example of an attestation." ;
    rdfs:subClassOf [ a owl:Restriction ;
            owl:allValuesFrom :Attester ;
            owl:onProperty :isMadeBy ],
        [ a owl:Restriction ;
            owl:allValuesFrom :Claim ;
            owl:onProperty :hasSubject ],
        lrml:Statement,
        :Substantiation ;
    skos:definition "An indefeasible statement, usually formal, made by an entity according to which they have witnessed or been presented with sufficient evidence to consider a specific claim made by another entity as truthful or accurate." .

:IdentityClaim a owl:Class ;
    rdfs:label "Identity Claim" ;
    rdfs:subClassOf :Claim ;
    skos:definition "A statement made by a claimant about their identity, usually with reference to some identification system." .

:Report a owl:Class ;
    rdfs:label "Report" ;
    rdfs:subClassOf :Claim ;
    skos:definition "A claim made according to some specification." .

:comprisesClaims a owl:ObjectProperty ;
    rdfs:label "comprisesClaims" ;
    rdfs:domain :Claim ;
    rdfs:range :Claim .

:hasObject a owl:ObjectProperty ;
    rdfs:label "hasObject" ;
    rdfs:domain :Claim ;
    rdfs:range :Object .

:hasPredicate a owl:ObjectProperty ;
    rdfs:label "hasPredicate" ;
    rdfs:domain :Claim ;
    rdfs:range :Predicate .

:Attester a owl:Class ;
    rdfs:label "Attester" ;
    skos:definition "An entity (e.g., a person, an organisation or a system) that makes an attestation." .

:Claimant a owl:Class ;
    rdfs:label "Claimant" ;
    skos:definition "An entity (e.g., a person, an organisation or a system) that makes a claim." .

:Object a owl:Class ;
    rdfs:label "Object" ;
    skos:definition "The target or value associated with the predicate of a claim or an attestation." .

:Predicate a owl:Class ;
    rdfs:label "Predicate" ;
    skos:definition "The characteristic, attribute, or relationship asserted about the subject of a claim or an attestation." .

:Subject a owl:Class ;
    rdfs:label "Subject" ;
    owl:equivalentClass owl:Thing ;
    skos:definition "The thing about which a statement (i.e., a claim or an attestation) is made." .

:isSupportedBy a owl:ObjectProperty ;
    rdfs:label "isSupportedBy" ;
    rdfs:domain :Claim ;
    rdfs:range :Substantiation ;
    owl:inverseOf :supports ;
    skos:definition "Indicates that a claim is backed or reinforced by some form of substantiation or evidence." .

:supports a owl:ObjectProperty ;
    rdfs:label "supports" ;
    rdfs:domain :Substantiation ;
    rdfs:range :Claim ;
    owl:inverseOf :isSupportedBy ;
    skos:definition "Indicates that a substantiation provides evidence or backing for a particular claim." .

:hasSubject a owl:ObjectProperty ;
    rdfs:label "hasSubject" ;
    rdfs:comment "This property is used on the Claim and Attestation classes. For a Claim the value assigned to this property must be a Subject; for an Attestation the value must be a Claim. This is enforced by owl:Restriction (see the definitions of the Claim and Attestation classes.)" .

:isMadeBy a owl:ObjectProperty ;
    rdfs:label "isMadeBy" ;
    rdfs:comment "This property is used on the Claim and Attestation classes. For a Claim the value assigned to this property must be a Claimant; for an Attestation the value must be an Attester. This is enforced by owl:Restriction (see the definitions of the Claim and Attestation classes.)" .

:Substantiation a owl:Class ;
    rdfs:label "Substantiation" ;
    skos:definition "A thing presented in support of the truthfulness of a claim." .

:Claim a owl:Class ;
    rdfs:label "Claim" ;
    rdfs:comment "A Claim may comprise other Claims." ;
    rdfs:subClassOf [ a owl:Restriction ;
            owl:allValuesFrom :Claimant ;
            owl:onProperty :isMadeBy ],
        [ a owl:Restriction ;
            owl:allValuesFrom :Subject ;
            owl:onProperty :hasSubject ],
        lrml:Statement ;
    skos:definition "A defeasible statement about a thing." .

[] a owl:AllDisjointClasses ;
    owl:members ( :Claim :Substantiation ) .

